Almost closed proof of fork rule

fairis/resources.v
@@ -1032,17 +1032,13 @@ Section model_state_lemmas.
       has_fuels ζ fs ∗ model_state_interp c2.1 δ2.
   Proof.
     iIntros (Hdom Hstep) "Hfuel Hm".
-    (* 1: Construct new model state *)
     iExists (model_update_locale_fuel (trace_last auxtr) ζ (dom fs)).
-    (* 2: Determine that we can step to new state *)
     iDestruct (model_state_interp_can_fuel_step with "Hm Hfuel") as %Hcan_step;
       [done|].
-    (* 3: Update ghost state in tandem with model state *)
     iMod (model_state_interp_fuel_update with "Hm Hfuel") as "[Hm Hfuel]";
       [done..|].
     iDestruct (model_state_interp_tids_smaller with "Hm") as %Htids.
     iModIntro.
-    (* 4: Close proof *)
     iFrame "Hm Hfuel".
     iPureIntro. by apply model_update_locale_spec.
   Qed.
@@ -1421,72 +1417,1013 @@ Section model_state_lemmas.
   (** Fork step *)
 
   Definition has_forked (tp1 tp2 : list (expr Λ)) e : Prop :=
-    ∃ tp1', tp2 = tp1' ++ [e] ∧ length tp1' = length tp1.
+    ∃ tp1', tp2 = tp1' ++ [e] ∧ locales_equiv tp1 tp1'.
 
-  (* OBS: Def might be improved. *)
-  (* OBS: Need freshness condition on ζf. *)
-  Program Definition model_update_split
-          (ζ ζf : locale Λ) (ρs : gset (fmrole M)) (δ : LM) : LM :=
-    {|
-      ls_data :=
-        {| ls_under := δ.(ls_under);
-           ls_map := <[ζf := filter (λ ρf, ρf.1 ∉ ρs) (δ.(ls_map) !!! ζ)]>
-                       (alter (filter (λ ρf, ρf.1 ∈ ρs)) ζ δ.(ls_map)); |};
-    |}.
-  Next Obligation. Admitted.
-  Next Obligation. Admitted.
+  Definition model_update_split
+             (ζ ζf : locale Λ) (ρs : gset (fmrole M))
+             (δ : LiveStateData Λ M) : LiveStateData Λ M :=
+    {| ls_under := δ.(ls_under);
+       ls_map := <[ζf := (filter (λ ρf, ρf.1 ∈ ρs)) (δ.(ls_map) !!! ζ)]>
+                   (alter (filter (λ ρf, ρf.1 ∉ ρs)) ζ δ.(ls_map)); |}.
 
-  (* OBS: Def needs to change to reflect forks *)
+  Definition map_live (ρs : gset (fmrole M))
+             (m : gmap (locale Λ) (gmap (fmrole M) nat)) : Prop :=
+    ∀ ρ, ρ ∈ ρs → ∃ ζ fs, m !! ζ = Some fs ∧ ρ ∈ dom fs.
+
+  Lemma disjoint_subseteq `{Countable A} (xs1 xs2 ys1 ys2 : gset A) :
+    xs1 ⊆ xs2 → ys1 ⊆ ys2 → xs2 ## ys2 → xs1 ## ys1.
+  Proof.
+    intros Hle1 Hle2 Hdisj x Hxs Hys.
+    eapply Hdisj; [by apply Hle1|by apply Hle2].
+  Qed.
+
+  Lemma disjoint_subseteq_l `{Countable A} (xs ys zs : gset A) :
+    xs ⊆ ys → ys ## zs → xs ## zs.
+  Proof. intros Hle Hdisj x Hxs Hzs. eapply Hdisj; [by apply Hle|done]. Qed.
+
+  Lemma disjoint_subseteq_r `{Countable A} (xs ys zs : gset A) :
+    zs ⊆ ys → xs ## ys → xs ## zs.
+  Proof. intros Hle Hdisj x Hxs Hzs. eapply Hdisj; [done|by apply Hle]. Qed.
+
+  (* Ugh *)
+  Lemma model_update_split_valid ζ ζf ρs (δ1 : LM) :
+    ζ ∈ dom δ1.(ls_map) → ζf ∉ dom δ1.(ls_map) →
+    ∃ δ2, (ls_data δ2) = model_update_split ζ ζf ρs δ1.
+  Proof.
+    intros [ρs' HSome]%elem_of_dom Hnin.
+    set δ2 := model_update_split ζ ζf ρs δ1.
+    assert (ζ ≠ ζf) as Hneq.
+    { intros ->. apply not_elem_of_dom in Hnin. set_solver. }
+    assert (map_inner_disj δ2.(ls_map)) as Hdisj.
+    { simpl.
+      pose proof δ1.(ls_map_disj) as Hdisj.
+      intros ζ1 ζ2 ρs1 ρs2 Hneq' HSome1 HSome2.
+      destruct (decide (ζf = ζ1)) as [<-|Hneqf1].
+      { rewrite lookup_insert in HSome1.
+        rewrite lookup_insert_ne in HSome2; [|done].
+        rewrite lookup_total_alt in HSome1.
+        rewrite HSome in HSome1.
+        simpl in *.
+        destruct (decide (ζ = ζ2)) as [<-|Hneq2].
+        { rewrite lookup_alter in HSome2.
+          rewrite HSome in HSome2. simpl in *. simplify_eq.
+          apply map_disjoint_dom.
+          pose proof (disjoint_filter_complement
+                        (λ ρ : fmrole M, ρ ∈ ρs) (dom ρs')) as Hcomp.
+          by rewrite !filter_dom_L in Hcomp. }
+        rewrite lookup_alter_ne in HSome2; [|done].
+        simplify_eq.
+        apply map_disjoint_dom.
+        pose proof (Hdisj ζ ζ2 _ _ Hneq2 HSome HSome2) as Hdisj.
+        apply map_disjoint_dom in Hdisj.
+        eapply disjoint_subseteq_l; [|done].
+        apply dom_filter_subseteq. }
+      rewrite lookup_insert_ne in HSome1; [|done].
+      destruct (decide (ζf = ζ2)) as [<-|Hneqf2].
+      { rewrite lookup_insert in HSome2.
+        destruct (decide (ζ = ζ1)) as [<-|Hneq2].
+        { rewrite lookup_alter in HSome1.
+          rewrite lookup_total_alt in HSome2.
+          rewrite HSome in HSome1.
+          rewrite HSome in HSome2.
+          simpl in *. simplify_eq.
+          apply map_disjoint_dom.
+          pose proof (disjoint_filter_complement
+                        (λ ρ : fmrole M, ρ ∈ ρs) (dom ρs')) as Hcomp.
+          by rewrite !filter_dom_L in Hcomp. }
+        rewrite lookup_alter_ne in HSome1; [|done].
+        rewrite lookup_total_alt in HSome2.
+        rewrite HSome in HSome2.
+        simpl in *. simplify_eq.
+        pose proof (Hdisj ζ ζ1 _ _ Hneq2 HSome HSome1) as Hdisj.
+        apply map_disjoint_dom.
+        apply map_disjoint_dom in Hdisj.
+        eapply disjoint_subseteq_r; [|done].
+        apply dom_filter_subseteq. }
+      destruct (decide (ζ = ζ1)) as [<-|Hneq1].
+      { rewrite lookup_alter in HSome1.
+        rewrite lookup_insert_ne in HSome2; [|done].
+        rewrite lookup_alter_ne in HSome2; [|done].
+        rewrite HSome in HSome1.
+        simpl in *. simplify_eq.
+        pose proof (Hdisj ζ ζ2 _ _ Hneq' HSome HSome2) as Hdisj.
+        apply map_disjoint_dom.
+        apply map_disjoint_dom in Hdisj.
+        eapply disjoint_subseteq_l; [|done].
+        apply dom_filter_subseteq. }
+      destruct (decide (ζ = ζ2)) as [<-|Hneq2].
+      { rewrite lookup_alter_ne in HSome1; [|done].
+        rewrite lookup_insert_ne in HSome2; [|done].
+        rewrite lookup_alter in HSome2.
+        rewrite HSome in HSome2.
+        simpl in *. simplify_eq.
+        pose proof (Hdisj ζ ζ1 _ _ Hneq1 HSome HSome1) as Hdisj.
+        apply map_disjoint_dom.
+        apply map_disjoint_dom in Hdisj.
+        eapply disjoint_subseteq_r; [|done].
+        apply dom_filter_subseteq. }
+      rewrite lookup_alter_ne in HSome1; [|done].
+      rewrite lookup_insert_ne in HSome2; [|done].
+      rewrite lookup_alter_ne in HSome2; [|done].
+      pose proof (Hdisj ζ1 ζ2 _ _ Hneq' HSome1 HSome2).
+      done. }
+    assert (map_live (M.(live_roles) δ2) δ2.(ls_map)) as Hlive.
+    { intros ρ Hin.
+      pose proof (δ1.(ls_map_live)) as Hlive.
+      apply Hlive in Hin as (ζ'&fs&HSome'&Hin').
+      destruct (decide (ζ' = ζf)) as [->|Hneqf].
+      { apply not_elem_of_dom in Hnin. set_solver. }
+      destruct (decide (ζ' = ζ)) as [->|Hneq'].
+      { rewrite HSome in HSome'. simplify_eq.
+        simpl.
+        destruct (decide (ρ ∈ ρs)) as [Hin|Hnin'].
+        - exists ζf, (filter (λ ρf : fmrole M * nat, ρf.1 ∈ ρs) fs).
+          rewrite lookup_insert. rewrite lookup_total_alt. rewrite HSome. simpl.
+          split; [done|].
+          apply elem_of_dom. rewrite /is_Some.
+          apply elem_of_dom in Hin' as [??].
+          eexists _. by apply map_filter_lookup_Some_2.
+        - exists ζ, (filter (λ ρf : fmrole M * nat, ρf.1 ∉ ρs) fs).
+          rewrite lookup_insert_ne; [|done].
+          rewrite lookup_alter. rewrite HSome. simpl.
+          split; [done|].
+          apply elem_of_dom. rewrite /is_Some.
+          apply elem_of_dom in Hin' as [??].
+          eexists _. by apply map_filter_lookup_Some_2. }
+      exists ζ', fs. split; [|done].
+      simpl. rewrite !lookup_insert_ne; [|done].
+      rewrite lookup_alter_ne; [|done].
+      done. }
+    by exists
+      {| ls_data := δ2;
+         ls_map_disj := Hdisj;
+         ls_map_live := Hlive |}.
+  Qed.
+
   Definition model_update_fork
-          (δ : LM) (ζ : locale Λ) (ζf : locale Λ) (ρs1 ρs2 : gset (fmrole M)) : LM :=
-    model_update_split ζ ζf ρs2 $ model_update_decr ζ $ model_update_filter ζ ρs1 δ.
+          (ζ : locale Λ) (ζf : locale Λ)
+          (ρs1 ρs2 : gset (fmrole M)) (δ : LM) :
+      LiveStateData Λ M :=
+    model_update_split ζ ζf ρs2 $
+    model_update_decr ζ $
+    model_update_filter ζ ρs1 δ.
+
+  (* Ugh *)
+  Lemma model_update_fork_valid
+        ζ ζf (ρs1 ρs2 : gset (fmrole M)) (δ1 : LM) :
+    ζ ∈ dom δ1.(ls_map) → ζf ∉ dom δ1.(ls_map) →
+    ∃ δ2, (ls_data δ2) = model_update_fork ζ ζf ρs1 ρs2 δ1.
+  Proof. intros ??. by apply model_update_split_valid; set_solver. Qed.
+
+  Lemma has_fuels_alloc fm ζ fs :
+    ζ ∉ dom fm →
+    auth_fuel_mapping_is fm ==∗
+    auth_fuel_mapping_is (<[ζ := fs]>fm) ∗ has_fuels ζ fs.
+  Proof.
+    iIntros (Hnin) "Hfm".
+    rewrite /has_fuels_S.
+    iMod (own_update with "Hfm") as "[$ $]"; [|done].
+    apply auth_update_alloc.
+    rewrite !fmap_insert.
+    rewrite !fmap_empty.
+    eapply alloc_local_update; [|done].
+    apply not_elem_of_dom in Hnin. by rewrite lookup_fmap Hnin.
+  Qed.
+
+
+  Lemma has_fuels_split fm ζ ζf fs1 fs2 :
+    ζf ∉ dom fm → fs1 ##ₘ fs2 →
+    auth_fuel_mapping_is fm -∗ has_fuels ζ (fs1 ∪ fs2) ==∗
+    auth_fuel_mapping_is (<[ζf := fs2]>(<[ζ := fs1]>fm)) ∗
+    has_fuels ζ fs1 ∗ has_fuels ζf fs2.
+  Proof.
+    iIntros (Hnin Hdisj) "Hfm Hfs".
+    iDestruct (has_fuels_agree with "Hfm Hfs") as %HSome.
+    assert (ζ ≠ ζf) as Hneq.
+    { rewrite not_elem_of_dom in Hnin. set_solver. }
+    iMod (has_fuels_update with "Hfm Hfs") as "[Hfm $]".
+    iMod (has_fuels_alloc with "Hfm") as "[$$]"; set_solver.
+  Qed.
+
+
+
+  Definition map_agree_R `{∀ A, Lookup K A (MAP A)} {A B}
+             (R : A → B → Prop) (m1 : MAP A) (m2 : MAP B) :=
+    map_relation R (λ _, False) (λ _, False) m1 m2.
+
+  Lemma map_agree_R_spec `{∀ A, Lookup K A (MAP A)} {A}
+        (R : relation A) (m1 m2 : MAP A) :
+    map_agree_R R m1 m2 ↔
+    (∀ k v1, m1 !! k = Some v1 → ∃ v2, m2 !! k = Some v2 ∧ R v1 v2) ∧
+    (∀ k v2, m2 !! k = Some v2 → ∃ v1, m1 !! k = Some v1 ∧ R v1 v2).
+  Proof.
+    rewrite /map_agree_R /map_relation /option_relation. split.
+    - intros HR. split.
+      + intros k v HSome. specialize (HR k). rewrite HSome in HR.
+        destruct (m2 !! k); [by eauto|done].
+      + intros k v HSome. specialize (HR k). rewrite HSome in HR.
+        destruct (m1 !! k); [by eauto|done].
+    - intros [HR1 HR2] k.
+      destruct (m1 !! k) as [v1|] eqn:Heqn1.
+      { by apply HR1 in Heqn1 as [? [-> ?]]. }
+      destruct (m2 !! k) as [v2|] eqn:Heqn2.
+      { apply HR2 in Heqn2 as [? [? ?]]. by simplify_eq. }
+      done.
+  Qed.
+
+  (* Lemma map_included_insert_inv `{Countable K} {V} *)
+  (*     (R : relation V) (m1 m2 : gmap K V) k v1 : *)
+  (*   map_included R (<[k:=v1]>m1) m2 → *)
+  (*   ∃ m2' v2, m2 = <[k:=v2]>m2' ∧ k ∉ dom m2' ∧ R v1 v2. *)
+  (* Proof. Admitted. *)
+
+  (* Lemma map_included_insert_inv `{Countable K} {V} *)
+  (*     (R : relation V) (m1 m2 : gmap K V) k v1 v2 : *)
+  (*   k ∉ dom m1 → k ∉ dom m2 → *)
+  (*   map_included R (<[k:=v1]>m1) (<[k:=v2]>m2) → *)
+  (*   map_included R m1 m2. *)
+  (* Proof. Admitted. *)
+
+  (* Lemma map_included_insert_inv_r `{Countable K} {V} *)
+  (*     (R : relation V) (m1 m2 : gmap K V) k v : *)
+  (*   k ∉ dom m1 → *)
+  (*   map_included R m1 (<[k:=v]> m2) → *)
+  (*   map_included R m1 m2. *)
+  (* Proof. Admitted. *)
+
+  Lemma map_included_delete `{Countable K} {V}
+      (R : relation V) (m1 m2 : gmap K V) k :
+    map_included R m1 m2 →
+    map_included R (delete k m1) (delete k m2).
+  Proof.
+    rewrite !map_included_spec.
+    intros Hle k' v HSome.
+    apply lookup_delete_Some in HSome as [HK HSome].
+    apply Hle in HSome as (?&?&?).
+    exists x. by rewrite lookup_delete_ne.
+  Qed.
+
+  Lemma map_agree_R_dom `{Countable K} {V}
+      (R : relation V) (m1 m2 : gmap K V) :
+    map_agree_R R m1 m2 → dom m1 = dom m2.
+  Proof.
+    rewrite map_agree_R_spec. intros [Hle1 Hle2]. apply set_eq.
+    intros k. split.
+    - intros [v1 HSome1]%elem_of_dom.
+      apply Hle1 in HSome1 as (?&?&?).
+      by apply elem_of_dom.
+    - intros [v2 HSome2]%elem_of_dom.
+      apply Hle2 in HSome2 as (?&?&?).
+      by apply elem_of_dom.
+  Qed.
+
+  Lemma map_agree_R_insert `{Countable K} {V}
+      (R : relation V) (m1 m2 : gmap K V) k v1 v2 :
+    R v1 v2 →
+    map_agree_R R m1 m2 →
+    map_agree_R R (<[k:=v1]>m1) (<[k:=v2]>m2).
+  Proof.
+    rewrite !map_agree_R_spec.
+    intros HR [Hle1 Hle2].
+    split.
+    - intros k' v1' HSome1.
+      destruct (decide (k = k')) as [->|Hneq].
+      + rewrite lookup_insert in HSome1. simplify_eq.
+        exists v2. rewrite lookup_insert. done.
+      + rewrite lookup_insert_ne in HSome1; [|done].
+        apply Hle1 in HSome1 as (v2'&HSome2&HR2).
+        exists v2'. rewrite lookup_insert_ne; [|done]. done.
+    - intros k' v2' HSome2.
+      destruct (decide (k = k')) as [->|Hneq].
+      + rewrite lookup_insert in HSome2. simplify_eq.
+        exists v1. rewrite lookup_insert. done.
+      + rewrite lookup_insert_ne in HSome2; [|done].
+        apply Hle2 in HSome2 as (v1'&HSome1&HR1).
+        exists v1'. rewrite lookup_insert_ne; [|done]. done.
+  Qed.
+
+  Lemma map_agree_R_insert_inv `{Countable K} {V}
+      (R : relation V) (m1 m2 : gmap K V) k v1 v2 :
+    k ∉ dom m1 → k ∉ dom m2 →
+    map_agree_R R (<[k:=v1]>m1) (<[k:=v2]>m2) →
+    map_agree_R R m1 m2.
+  Proof.
+    intros Hnin1 Hnin2.
+    rewrite !map_agree_R_spec.
+    intros [Hle1 Hle2].
+    split.
+    - intros k' v1' HSome1.
+      destruct (decide (k = k')) as [->|Hneq].
+      { apply not_elem_of_dom in Hnin1. set_solver. }
+      assert (<[k:=v1]>m1 !! k' = Some v1') as HSome1'.
+      { by rewrite lookup_insert_ne. }
+      apply Hle1 in HSome1' as (v2'&HSome2&HR).
+      rewrite lookup_insert_ne in HSome2; [|done].
+      by eauto.
+    - intros k' v2' HSome2.
+      destruct (decide (k = k')) as [->|Hneq].
+      { apply not_elem_of_dom in Hnin2. set_solver. }
+      assert (<[k:=v2]>m2 !! k' = Some v2') as HSome2'.
+      { by rewrite lookup_insert_ne. }
+      apply Hle2 in HSome2' as (v1'&HSome1&HR).
+      rewrite lookup_insert_ne in HSome1; [|done].
+      by eauto.
+  Qed.
+
+  Lemma map_agree_R_agree `{Countable K} {V}
+      (R : relation V) (m1 m2 : gmap K V) k v1 v2 :
+    m1 !! k = Some v1 → m2 !! k = Some v2 →
+    map_agree_R R m1 m2 →
+    R v1 v2.
+  Proof.
+    rewrite map_agree_R_spec.
+    intros HSome1 HSome2 Hle.
+    apply Hle in HSome1 as (v2'&HSome2'&HR).
+    rewrite HSome2' in HSome2. by simplify_eq.
+  Qed.
+
+  Lemma map_included_R_agree `{Countable K} {V}
+      (R : relation V) (m1 m2 : gmap K V) k v1 v2 :
+    m1 !! k = Some v1 → m2 !! k = Some v2 →
+    map_included R m1 m2 →
+    R v1 v2.
+  Proof.
+    rewrite map_included_spec.
+    intros HSome1 HSome2 Hle.
+    apply Hle in HSome1 as (v2'&HSome2'&HR).
+    rewrite HSome2' in HSome2. by simplify_eq.
+  Qed.
+
+  Lemma map_included_map_agree_R `{Countable K} {V}
+      (R : relation V) (m1 m2 : gmap K V) :
+    map_included R m1 m2 →
+    ∃ m21 m22,
+      m2 = m21 ∪ m22 ∧
+      m21 ##ₘ m22 ∧
+      map_agree_R R m1 m21.
+  Proof.
+    revert m1.
+    induction m2 as [|k v2 m2 Hnin IHm2] using map_ind; intros m1 Hle.
+    { by exists ∅, ∅. }
+    destruct (decide (k ∈ dom m1)) as [Hin|Hnin']; last first.
+    { apply (map_included_delete _ _ _ k) in Hle.
+      rewrite delete_insert in Hle; [|done].
+      apply IHm2 in Hle as (m21&m22&->&Hdisj&HR).
+      exists m21, (<[k:=v2]>m22).
+      assert (dom m1 = dom m21) as Hdom.
+      { eapply map_agree_R_dom. apply not_elem_of_dom in Hnin'.
+        by rewrite delete_notin in HR. }
+      apply map_disjoint_dom in Hdisj.
+      rewrite insert_union_r; [|by apply not_elem_of_dom; set_solver].
+      split; [done|].
+      apply not_elem_of_dom in Hnin'.
+      rewrite delete_notin in HR; [|done].
+      split; [|done].
+      apply map_disjoint_dom.
+      apply not_elem_of_dom in Hnin'.
+      set_solver. }
+    apply elem_of_dom in Hin as [v1 HSome].
+    assert (R v1 v2).
+    { eapply map_included_R_agree; [| |done].
+      - done.
+      - by rewrite lookup_insert. }
+    apply (map_included_delete _ _ _ k) in Hle.
+    rewrite delete_insert in Hle; [|done].
+    apply IHm2 in Hle as (m21&m22&->&Hdisj&HR).
+    exists (<[k:=v2]>m21), m22.
+    assert (dom (delete k m1) = dom m21) as Hdom.
+    { eapply map_agree_R_dom. done. }
+    apply map_disjoint_dom in Hdisj.
+    rewrite insert_union_l.
+    split; [done|].
+    apply (map_agree_R_insert _ _ _ k v1 v2) in HR; [|done].
+    rewrite insert_delete in HR; [|done].
+    split; [|done].
+    apply map_disjoint_dom.
+    rewrite dom_insert_L.
+    apply not_elem_of_dom in Hnin.
+    set_solver.
+  Qed.
+
+  Lemma map_agree_R_map_included `{Countable K} {V}
+      (R : relation V) (m1 m2 : gmap K V) :
+    map_agree_R R m1 m2 → map_included R m1 m2.
+  Proof.
+    rewrite map_included_spec map_agree_R_spec.
+    by intros [Hle _].
+  Qed.
+
+  (* Lemma map_agree_R_refl `{Countable K} {V} *)
+  (*     (R : relation V) `{!Reflexive R} (m : gmap K V) : *)
+  (*   map_agree_R R m m. *)
+  (* Proof. *)
+  (*   rewrite map_agree_R_spec. *)
+  (*   induction m as [|k v m Hnin Hm] using map_ind; [done|]. *)
+  (*   split. *)
+  (*   - intros k' v1 HSome1. *)
+  (*     destruct (decide (k = k')) as [->|Hneq]. *)
+  (*     + rewrite lookup_insert in HSome1. *)
+  (*       simplify_eq. *)
+  (*       exists v1. rewrite lookup_insert. done. *)
+  (*     + admit. *)
+  (*   - admit. *)
+  (* Admitted. *)
+
+  Lemma map_agree_R_union_inv `{Countable K} {V}
+      (R : relation V) (m11 m12 m2 : gmap K V) :
+    m11 ##ₘ m12 →
+    map_agree_R R (m11 ∪ m12) m2 →
+    ∃ m21 m22, m2 = m21 ∪ m22 ∧ map_agree_R R m11 m21 ∧
+               map_agree_R R m12 m22.
+  Proof.
+    intros Hdisj%map_disjoint_dom Hle.
+    pose proof Hle as Hdom%map_agree_R_dom.
+    rewrite comm in Hdom.
+    rewrite dom_union_L in Hdom.
+    apply dom_union_inv_L in Hdom as (m21&m22&->&Hdosj&Hdom1&Hdom2);
+      [|done].
+    exists m21, m22.
+    split; [done|].
+    split.
+    - apply map_agree_R_spec.
+      split.
+      + intros k v1 HSome1.
+        apply map_agree_R_spec in Hle as [Hle1 Hle2].
+        assert ((m11 ∪ m12) !! k = Some v1) as HSome1'.
+        { rewrite lookup_union_l; [done|].
+          apply not_elem_of_dom.
+          apply elem_of_dom_2 in HSome1. set_solver. }
+        apply Hle1 in HSome1' as (v2&HSome2'&HR).
+        assert (m21 !! k = Some v2) as HSome2.
+        { rewrite lookup_union_l in HSome2'; [done|].
+          apply not_elem_of_dom. apply elem_of_dom_2 in HSome1.
+          set_solver. }
+        eauto.
+      + intros k v2 HSome2.
+        apply map_agree_R_spec in Hle as [Hle1 Hle2].
+        assert ((m21 ∪ m22) !! k = Some v2) as HSome2'.
+        { rewrite lookup_union_l; [done|].
+          apply not_elem_of_dom.
+          apply elem_of_dom_2 in HSome2. set_solver. }
+        apply Hle2 in HSome2' as (v1&HSome1'&HR).
+        assert (m11 !! k = Some v1) as HSome1.
+        { rewrite lookup_union_l in HSome1'; [done|].
+          apply not_elem_of_dom. apply elem_of_dom_2 in HSome2.
+          set_solver. }
+        eauto.
+    - apply map_agree_R_spec.
+      split.
+      + intros k v1 HSome1.
+        apply map_agree_R_spec in Hle as [Hle1 Hle2].
+        assert ((m11 ∪ m12) !! k = Some v1) as HSome1'.
+        { rewrite lookup_union_r; [done|].
+          apply not_elem_of_dom.
+          apply elem_of_dom_2 in HSome1. set_solver. }
+        apply Hle1 in HSome1' as (v2&HSome2'&HR).
+        assert (m22 !! k = Some v2) as HSome2.
+        { rewrite lookup_union_r in HSome2'; [done|].
+          apply not_elem_of_dom. apply elem_of_dom_2 in HSome1.
+          set_solver. }
+        eauto.
+      + intros k v2 HSome2.
+        apply map_agree_R_spec in Hle as [Hle1 Hle2].
+        assert ((m21 ∪ m22) !! k = Some v2) as HSome2'.
+        { rewrite lookup_union_r; [done|].
+          apply not_elem_of_dom.
+          apply elem_of_dom_2 in HSome2. set_solver. }
+        apply Hle2 in HSome2' as (v1&HSome1'&HR).
+        assert (m12 !! k = Some v1) as HSome1.
+        { rewrite lookup_union_r in HSome1'; [done|].
+          apply not_elem_of_dom. apply elem_of_dom_2 in HSome2.
+          set_solver. }
+        eauto.
+  Qed.
+
+  (* OBS: Need restrictions on f *)
+  Lemma map_agree_R_fmap_inv `{Countable K} {V}
+      (R : relation V) (m1 m2 : gmap K V) f :
+    (* OBS: Is this a general relation/function property? *)
+    (∀ v1 v2, R (f v1) v2 → ∃ v2', v2 = f v2') →
+    map_agree_R R (f <$> m1) m2 →
+    ∃ m2', m2 = f <$> m2'.
+  Proof.
+    revert m1.
+    induction m2 as [|k v2 m2 Hnin IHm2] using map_ind; intros m1 Hf Hle.
+    { exists ∅. rewrite fmap_empty. done. }
+    pose proof Hle as Hle'.
+    apply map_agree_R_spec in Hle.
+    assert (<[k:=v2]> m2 !! k = Some v2) as HSome2
+           by by rewrite lookup_insert.
+    apply Hle in HSome2 as (v1&HSome1&HR).
+    apply lookup_fmap_Some in HSome1 as (v1'&<-&HSome1').
+    assert (∃ v2', v2 = f v2') as [v2' Heq].
+    { by eapply Hf. }
+    rewrite Heq in HR.
+    assert (map_agree_R R (f <$> (delete k m1)) m2) as Hle''.
+    { rewrite -(insert_id m1 k v1') in Hle'; [|done].
+      rewrite -insert_delete_insert in Hle'.
+      rewrite fmap_insert in Hle'.
+      eapply map_agree_R_insert_inv; [| |apply Hle'].
+      - set_solver.
+      - apply not_elem_of_dom. set_solver.
+    }
+    apply IHm2 in Hle'' as [m2' Heq']; [|done].
+    exists (<[k:=v2']>m2').
+    rewrite fmap_insert. rewrite Heq. f_equiv. done.
+  Qed.
+
+  (* OBS: Need restrictions on f *)
+  Lemma map_agree_R_fmap `{Countable K} {V}
+      (R : relation V) (m1 m2 : gmap K V) f :
+    (∀ v1 v2, R (f v1) (f v2) → R v1 v2) →
+    map_agree_R R (f <$> m1) (f <$> m2) →
+    map_agree_R R m1 m2.
+  Proof.
+    intros Hf.
+    rewrite !map_agree_R_spec.
+    intros [Hle1 Hle2].
+    split.
+    - intros k v1 HSome1.
+      assert ((f <$> m1) !! k = Some (f v1)) as HSome1'.
+      { rewrite lookup_fmap. destruct (m1 !! k); [by simplify_eq|done]. }
+      apply Hle1 in HSome1' as (v2'&HSome2'&HR).
+      apply lookup_fmap_Some in HSome2' as (v2&<-&HSome2).
+      apply Hf in HR.
+      by eauto.
+    - intros k v2 HSome2.
+      assert ((f <$> m2) !! k = Some (f v2)) as HSome2'.
+      { rewrite lookup_fmap. destruct (m2 !! k); [by simplify_eq|done]. }
+      apply Hle2 in HSome2' as (v1'&HSome1'&HR).
+      apply lookup_fmap_Some in HSome1' as (v1&<-&HSome1).
+      apply Hf in HR.
+      by eauto.
+  Qed.
+
+  Lemma locale_of_from_list_from (tp0 tp0' tp tp' : list $ expr Λ) e :
+    locales_equiv tp0 tp0' →
+    locales_equiv tp tp' →
+    locale_of (tp0++tp) e ∉ locales_of_list_from tp0' tp'.
+  Proof. Admitted.
+
+  (* Lemma not_elem_of_locale_of_from_list (tp : list $ expr Λ) e : *)
+  (*   locale_of tp e ∉ locales_of_list tp. *)
+  (* Proof. *)
+  (*   rewrite -{1}(app_nil_l tp). *)
+  (*   apply locale_of_from_list_from; apply locales_equiv_refl. *)
+  (* Qed. *)
+
+  Lemma not_elem_of_locale_of_from_list (tp1 tp2 : list $ expr Λ) e :
+    locales_equiv tp1 tp2 →
+    locale_of tp1 e ∉ locales_of_list tp2.
+  Proof.
+    intros. rewrite -{1}(app_nil_l tp1).
+    apply locale_of_from_list_from; [apply locales_equiv_refl|done].
+  Qed.
+
+  Lemma elem_of_locale_of_from_list (tp1 tp2 : list $ expr Λ) e :
+    locales_equiv tp1 tp2 →
+    locale_of tp1 e ∈ locales_of_list (tp2++[e]).
+  Proof. Admitted.
 
   Lemma model_state_interp_fork_update fs1 fs2 tp1 tp2
-        δ ζ efork σ1 σ2 :
+        (δ1 δ2 : LM) ζ efork σ1 σ2 :
+    (ls_data δ2) = model_update_fork ζ (locale_of tp1 efork) (dom fs1 ∪ dom fs2) (dom fs2) δ1 →
     fs1 ∪ fs2 ≠ ∅ → fs1 ##ₘ fs2 →
+    has_forked tp1 tp2 efork →
     locale_step (tp1, σ1) (Some ζ) (tp2, σ2) →
-    model_state_interp tp1 δ -∗
+    model_state_interp tp1 δ1 -∗
     has_fuels_S ζ (fs1 ∪ fs2) ==∗
-    model_state_interp tp2
-      (model_update_fork δ ζ (locale_of tp1 efork)
-                                (dom (fs1 ∪ fs2)) (dom fs1)) ∗
+    model_state_interp tp2 δ2 ∗
     has_fuels ζ fs1 ∗
     has_fuels (locale_of tp1 efork) fs2.
-  Proof. Admitted.
+  Proof.
+    iIntros (Hδ2 Hfs Hdisj Hforked Hstep) "Hm Hf".
+    iDestruct "Hm" as (fm Hfmle Hfmdead Htp) "(Hm & Hfm)".
+    iDestruct (has_fuels_agree with "Hfm Hf") as %Hagree.
+    assert (locale_of tp1 efork ∉ dom fm) as Hnin.
+    { pose proof (not_elem_of_locale_of_from_list tp1 tp1 efork) as Hes%Htp; [|apply locales_equiv_refl].
+      apply not_elem_of_dom in Hes. set_solver. }
+    assert (ζ ≠ locale_of tp1 efork) as Hneq.
+    { rewrite not_elem_of_dom in Hnin. set_solver. }
+    iMod (has_fuels_decr with "Hfm Hf") as "[Hfm Hf]".
+    iMod (has_fuels_split _ _ (locale_of tp1 efork) with "Hfm Hf")
+      as "[Hfm [Hf1 Hf2]]"; [|done|].
+    { set_solver. }
+    iModIntro. iFrame. iExists _. iFrame. rewrite Hδ2. iFrame.
+    iPureIntro.
+    split; [|split].
+    - (* TODO: Find a good way to prove this *)
+      split; last first.
+      { simpl.
+        destruct Hfmle as [Hfmle Hdom].
+        pose proof Hfmle as Hfmle'.
+        rewrite /fuel_map_le /fuel_map_le_inner map_included_spec in Hfmle.
+        pose proof Hagree as Hagree'.
+        apply Hfmle in Hagree' as (fs'&HSome&Hfs').
+        rewrite -(insert_id (ls_map δ1) ζ fs'); [|done].
+        rewrite !alter_insert.
+        set_solver. }
+      simpl.
+      destruct Hfmle as [Hfmle Hdom].
+      pose proof Hfmle as Hfmle'.
+      rewrite /fuel_map_le /fuel_map_le_inner map_included_spec in Hfmle.
+      pose proof Hagree as Hagree'.
+      apply Hfmle in Hagree' as (fs'&HSome&Hfs').
+      rewrite -(insert_id (ls_map δ1) ζ fs'); [|done].
+      rewrite !alter_insert.
+      rewrite insert_insert.
+
+      apply map_included_map_agree_R in Hfs'
+          as (fs12'&fsf'&->&Hdisj'&Hfs').
+      pose proof Hfs' as Hfs''.
+      apply map_agree_R_fmap_inv in Hfs'' as [fs1'' ->]; last first.
+      { intros ?[]?; [lia|by eauto]. }
+      apply map_agree_R_fmap in Hfs'; last first.
+      { intros. lia. }
+      apply map_agree_R_union_inv in Hfs'
+          as (fs1'&fs2'&->&Hfs1'&Hfs2'); [|done].
+
+      apply map_included_insert.
+      { rewrite lookup_total_alt.
+        rewrite lookup_insert.
+        rewrite map_filter_fmap.
+        rewrite map_filter_filter.
+        rewrite map_fmap_union.
+        rewrite map_filter_union; last first.
+        { apply map_disjoint_dom. apply map_disjoint_dom in Hdisj'.
+          set_solver. }
+        rewrite map_filter_union; last first.
+        { apply map_disjoint_dom. apply map_disjoint_dom in Hdisj.
+          apply map_agree_R_dom in Hfs1'.
+          apply map_agree_R_dom in Hfs2'.
+          set_solver. }
+        rewrite !map_fmap_union.
+        eapply map_included_subseteq_r.
+        { apply map_union_subseteq_l. }
+        eapply map_included_subseteq_r.
+        { apply map_union_subseteq_r.
+          apply map_disjoint_dom.
+          rewrite !map_filter_fmap. rewrite !dom_fmap_L.
+          apply map_disjoint_dom in Hdisj.
+          apply map_agree_R_dom in Hfs1'.
+          apply map_agree_R_dom in Hfs2'.
+          eapply disjoint_subseteq_l; [apply dom_filter_subseteq|].
+          eapply disjoint_subseteq_r; [apply dom_filter_subseteq|].
+          set_solver. }
+        rewrite map_filter_id; last first.
+        { simpl.
+          intros. apply elem_of_dom_2 in H0.
+          apply map_agree_R_dom in Hfs1'.
+          apply map_agree_R_dom in Hfs2'.
+          split; [set_solver|].
+          set_solver. }
+        rewrite -map_fmap_compose.
+        rewrite decr_succ_compose_id. rewrite map_fmap_id.
+        by apply map_agree_R_map_included. }
+
+      apply map_included_insert; [|done].
+      rewrite map_filter_fmap.
+      rewrite map_filter_filter.
+
+      rewrite !map_fmap_union.
+      rewrite map_filter_union; last first.
+      { apply map_disjoint_dom. apply map_disjoint_dom in Hdisj'.
+        set_solver. }
+      rewrite map_filter_union; last first.
+      { apply map_disjoint_dom. apply map_disjoint_dom in Hdisj.
+        apply map_agree_R_dom in Hfs1'.
+        apply map_agree_R_dom in Hfs2'.
+        set_solver. }
+      rewrite !map_fmap_union.
+      eapply map_included_subseteq_r.
+      { apply map_union_subseteq_l. }
+      eapply map_included_subseteq_r.
+      { apply map_union_subseteq_l. }
+
+      rewrite map_filter_id; last first.
+      { simpl.
+        intros. apply elem_of_dom_2 in H0.
+        apply map_agree_R_dom in Hfs1'.
+        apply map_agree_R_dom in Hfs2'.
+        rewrite dom_fmap in H0.
+        apply map_disjoint_dom in Hdisj.
+        split; [set_solver|].
+        set_solver. }
+      rewrite -map_fmap_compose.
+      rewrite decr_succ_compose_id. rewrite map_fmap_id.
+      by apply map_agree_R_map_included.
+  - intros ρ' Hin.
+      apply Hfmdead in Hin as (ζ'&ρs&HSome&Hρ).
+      destruct (decide (ζ = ζ')) as [<-|Hneq'].
+      + rewrite Hagree in HSome.
+        simplify_eq.
+        rewrite dom_fmap_L in Hρ.
+        rewrite dom_union_L in Hρ.
+        apply elem_of_union in Hρ.
+        destruct Hρ as [Hρ|Hρ].
+        * eexists ζ, _. rewrite insert_insert.
+          rewrite insert_commute; [|done].
+          rewrite lookup_insert. done.
+        * eexists (locale_of tp1 efork), _. rewrite insert_insert.
+          rewrite lookup_insert. done.
+      + assert (ζ' ≠ locale_of tp1 efork) as Hneq''.
+        { intros ->. apply not_elem_of_dom in Hnin. set_solver. }
+        eexists ζ', _.
+        rewrite lookup_insert_ne; [|done].
+        rewrite insert_insert.
+        rewrite lookup_insert_ne; [|done].
+        split; [done|]. by set_solver.
+    - rewrite /fuel_map_preserve_threadpool.
+      intros ζ' Hζ'.
+      apply locales_of_list_step_incl in Hstep.
+      assert (ζ' ∉ locales_of_list tp1) as Hζ'' by set_solver.
+      apply Htp in Hζ''.
+      rewrite insert_insert.
+      assert (ζ ≠ ζ') as Hneq'.
+      { set_solver. }
+      assert (locale_of tp1 efork ≠ ζ') as Hneq''.
+      { assert (locale_of tp1 efork ∈ locales_of_list tp2).
+        { destruct Hforked as [tp2' [-> Hequiv]].
+          by apply elem_of_locale_of_from_list. }
+        set_solver. }
+      rewrite lookup_insert_ne; [|done].
+      rewrite lookup_insert_ne; [|done].
+      done.
+  Qed.
 
   (* TODO: Need to update this to reflect fork requirements. *)
-  Definition model_can_fork_step (δ1 : LM) (ζ : locale Λ) (δ2 : LM) : Prop :=
-    ∃ fs1 fs1',
+  Definition model_can_fork_step (δ1 : LM) (ζ ζf : locale Λ) (δ2 : LM) : Prop :=
+    ∃ fs fs1 fs2,
       δ1.(ls_under) = δ2.(ls_under) ∧
-      δ1.(ls_map) !! ζ = Some fs1 ∧
-      δ2.(ls_map) = <[ζ := fs1']>δ1.(ls_map) ∧
-      fs1 ≠ ∅ ∧
-      map_included (<) fs1' fs1 ∧
-      (dom fs1 ∖ dom fs1') ∩ M.(live_roles) δ1 = ∅.
+      δ1.(ls_map) !! ζ = Some fs ∧ fs ≠ ∅ ∧
+      δ2.(ls_map) = <[ζ := fs1]>(<[ζf := fs2]> δ1.(ls_map)) ∧
+      map_included (<) fs1 fs ∧
+      map_included (<) fs2 fs ∧
+      (dom fs ∖ (dom fs1 ∪ dom fs2) ∩ M.(live_roles) δ1 = ∅) ∧
+      (dom fs1 ∩ dom fs2 = ∅) ∧
+      ζf ∉ dom δ1.(ls_map).
 
-  Lemma model_can_fork_step_trans fl ζ (δ δ' : LiveState Λ M) :
-    model_can_fork_step δ ζ δ' → ls_trans fl δ (Silent_step ζ) δ'.
-  Proof. Admitted.
+  Lemma silent_step_suff_data_fork_weak fl `(δ: LiveState Λ M)
+        (fs fs1 fs2 : gmap _ nat) ζ ζf :
+    δ.(ls_map) !! ζ = Some fs →
+    fs ≠ ∅ →
+    map_included (<) fs1 fs →
+    map_included (<) fs2 fs →
+    (dom fs ∖ (dom fs1 ∪ dom fs2)) ∩ M.(live_roles) δ = ∅ →
+    (dom fs1 ∩ dom fs2 = ∅) →
+    ζf ∉ dom δ.(ls_map) →
+    ∃ δ', δ'.(ls_data) =
+          {| ls_under := δ;
+            ls_map := <[ζ := fs1]>(<[ζf := fs2]> δ.(ls_map)) |} ∧
+            ls_trans fl δ (Silent_step ζ) δ'.
+  Proof.
+    intros.
+    apply (silent_step_suff_data fl δ fs fs1 fs2 ζ (Some ζf)); try done.
+    - rewrite map_included_spec in H2. done.
+    - rewrite map_included_spec in H3. done.
+    - set_solver.
+  Qed.
 
-  Lemma model_state_interp_can_fork_step es δ ζ ζf
-        (fs1 fs2 : gmap (fmrole M) nat) :
+  (* TODO: Change original lemma to not existentially quantify new state *)
+  Lemma silent_step_suff_data_fork_weak_alt fl (δ δ': LiveState Λ M)
+        (fs fs1 fs2 : gmap _ nat) ζ ζf :
+    δ.(ls_under) = δ'.(ls_under) →
+    δ.(ls_map) !! ζ = Some fs →
+    δ'.(ls_map) = <[ζ := fs1]>(<[ζf := fs2]> δ.(ls_map)) →
+    fs ≠ ∅ →
+    map_included (<) fs1 fs →
+    map_included (<) fs2 fs →
+    (dom fs ∖ (dom fs1 ∪ dom fs2)) ∩ M.(live_roles) δ = ∅ →
+    (dom fs1 ∩ dom fs2 = ∅) →
+    ζf ∉ dom δ.(ls_map) →
+    ls_trans fl δ (Silent_step ζ) δ'.
+  Proof.
+    rewrite !map_included_spec.
+    intros Hδ Hfs Hfs12 Hne Hle1 Hle2 Hlive Hdisj Hnin.
+    assert (∃ δ', δ'.(ls_data) =
+          {| ls_under := δ;
+            ls_map := <[ζ := fs1]> (<[ζf := fs2]>δ.(ls_map)) |} ∧
+            ls_trans fl δ (Silent_step ζ) δ') as (δ''&Heq&Htrans).
+    { apply (silent_step_suff_data fl δ fs fs1 fs2 ζ (Some ζf));
+        try set_solver. }
+    rewrite Heq Hδ -Hfs12 in Htrans. by destruct δ', ls_data.
+  Qed.
+
+  Lemma model_can_fork_step_trans fl ζ ζf (δ δ' : LiveState Λ M) :
+    model_can_fork_step δ ζ ζf δ' → ls_trans fl δ (Silent_step ζ) δ'.
+  Proof.
+    destruct 1 as (?&?&?&?&?&?&?&?&?&?&?&?).
+    by eapply silent_step_suff_data_fork_weak_alt.
+  Qed.
+
+  Lemma model_state_interp_can_fork_step es (δ1 δ2 : LM) ζ
+        (fs1 fs2 : gmap (fmrole M) nat) e :
+    (ls_data δ2) = model_update_fork ζ (locale_of es e) (dom fs1 ∪ dom fs2) (dom fs2) δ1 →
     (fs1 ∪ fs2) ≠ ∅ → fs1 ##ₘ fs2 →
-    model_state_interp es δ -∗ has_fuels_S ζ (fs1 ∪ fs2) -∗
-    ⌜model_can_fork_step δ ζ (model_update_fork δ ζ ζf (dom (fs1 ∪ fs2)) (dom fs1))⌝.
-  Proof. Admitted.
+    model_state_interp es δ1 -∗ has_fuels_S ζ (fs1 ∪ fs2) -∗
+    ⌜model_can_fork_step δ1 ζ (locale_of es e) δ2⌝.
+  Proof.
+    iIntros (Hδ2 Hne Hdisj) "Hm Hf".
+    iDestruct "Hm" as (fm [Hfmle Hdom] Hfmdead Htp) "(Hm & Hfm)".
+    iDestruct (has_fuels_agree with "Hfm Hf") as %Hagree.
+    pose proof Hagree as Hagree'.
+    rewrite /fuel_map_le_inner map_included_spec in Hfmle.
+    apply Hfmle in Hagree as (fs'&HSome&Hle).
+    iPureIntro.
+    apply map_included_map_agree_R in Hle as (fs12'&fsf'&->&Hdisj'&Hle).
+    pose proof Hle as Hle'.
+    apply map_agree_R_fmap_inv in Hle' as (fs12''&->); last first.
+    { intros. destruct v2; [lia|by eauto]. }
+    apply map_agree_R_fmap in Hle; last first.
+    { intros. lia. }
+    apply map_agree_R_union_inv in Hle as (fs1'&fs2'&->&Hle1&Hle2);
+      [|done].
+    eexists _, fs1', fs2'.
+    repeat split.
+    - rewrite Hδ2. done.
+    - done.
+    - apply map_agree_R_dom in Hle1.
+      apply map_agree_R_dom in Hle2.
+      intros Heq. apply Hne.
+      apply dom_empty_iff_L in Heq.
+      apply dom_empty_iff_L.
+      set_solver.
+    - rewrite Hδ2. simpl.
+      rewrite insert_commute; last first.
+      { assert (locale_of es e ∉ locales_of_list es) as Hes%Htp.
+        { apply not_elem_of_locale_of_from_list.
+          apply locales_equiv_refl. }
+        set_solver. }
+      f_equiv.
+      { rewrite lookup_total_alt. simpl.
+        rewrite !lookup_alter. rewrite HSome.
+        simpl.
+        rewrite map_filter_fmap. simpl.
+        rewrite map_filter_filter. simpl.
+        rewrite !map_fmap_union.
+        apply map_agree_R_dom in Hle1.
+        apply map_agree_R_dom in Hle2.
+        apply map_disjoint_dom in Hdisj.
+        apply map_disjoint_dom in Hdisj'.
+        rewrite map_filter_union; [|apply map_disjoint_dom; set_solver].
+        rewrite map_filter_union; [|apply map_disjoint_dom; set_solver].
+        assert (filter
+                  (λ '(i, _),
+                     i ∈ dom fs2 ∧ (i ∈ live_roles M δ1 ∨ i ∈ dom fs1 ∪ dom fs2))
+                  (S <$> fs1') = ∅) as Hfs1'.
+        { apply map_filter_empty_iff.
+          intros ρ f Hρ [HP1 HP2].
+          apply elem_of_dom_2 in Hρ.
+          rewrite dom_fmap_L in Hρ. set_solver. }
+        assert (filter
+                  (λ '(i, _),
+                     i ∈ dom fs2 ∧ (i ∈ live_roles M δ1 ∨ i ∈ dom fs1 ∪ dom fs2))
+                  fsf' = ∅) as Hfsf'.
+        { apply map_filter_empty_iff.
+          intros ρ f Hρ [HP1 HP2].
+          apply elem_of_dom_2 in Hρ. set_solver. }
+        rewrite Hfs1' Hfsf'.
+        rewrite left_id right_id.
+        rewrite map_filter_id; last first.
+        { intros. split.
+          - apply elem_of_dom_2 in H0. set_solver.
+          - right.
+            apply elem_of_dom_2 in H0. set_solver. }
+        rewrite -map_fmap_compose.
+        rewrite decr_succ_compose_id.
+        rewrite map_fmap_id.
+        done. }
+      rewrite -!alter_compose.
+      erewrite alter_insert_alt; [|done].
+      f_equiv.
+      simpl.
+      rewrite map_filter_fmap. simpl.
+      rewrite map_filter_filter. simpl.
+      apply map_agree_R_dom in Hle1.
+      apply map_agree_R_dom in Hle2.
+      apply map_disjoint_dom in Hdisj.
+      apply map_disjoint_dom in Hdisj'.
+      rewrite !map_fmap_union.
+      rewrite map_filter_union; [|apply map_disjoint_dom; set_solver].
+      rewrite map_filter_union; [|apply map_disjoint_dom; set_solver].
+      assert (filter
+             (λ '(i, _),
+                (i ∉ dom fs2) ∧ (i ∈ live_roles M δ1 ∨ i ∈ dom fs1 ∪ dom fs2))
+             (S <$> fs2') = ∅) as Hfs2'.
+      { apply map_filter_empty_iff.
+        intros ρ f Hρ [HP1 HP2].
+        apply elem_of_dom_2 in Hρ.
+        rewrite dom_fmap_L in Hρ. set_solver. }
+      assert (filter
+                (λ '(i, _),
+                   (i ∉ dom fs2) ∧ (i ∈ live_roles M δ1 ∨ i ∈ dom fs1 ∪ dom fs2))
+                fsf' = ∅) as Hfsf'.
+      { apply map_filter_empty_iff.
+        intros ρ f Hρ [HP1 HP2].
+        apply elem_of_dom_2 in Hρ.
+        rewrite Hle2 in HP1.
+        clear HP1.
+        assert (ρ ∈ (dom fs1 ∪ dom fs2)).
+        { destruct HP2 as [HP2|?]; [|done].
+          rewrite -dom_union_L.
+          rewrite -(dom_fmap_L S).
+          eapply fuel_map_le_live_roles; [| | |apply Hagree'|..].
+          - intros ????. by apply δ1.(ls_map_disj).
+            (* TODO: Fix this by unifying defs *)
+          - rewrite /fuel_map_le_inner map_included_spec.
+            eapply Hfmle.
+          - done.
+          - done.
+          - done.
+          - set_solver. }
+        set_solver. }
+      rewrite Hfs2' Hfsf'.
+      rewrite right_id right_id.
+      rewrite map_filter_id; last first.
+      { intros. split.
+        - apply elem_of_dom_2 in H0. set_solver.
+        - right.
+          apply elem_of_dom_2 in H0. set_solver. }
+      rewrite -map_fmap_compose.
+      rewrite decr_succ_compose_id.
+      rewrite map_fmap_id.
+      done.
+    - eapply (map_included_subseteq_r _ _ (S <$> fs1')).
+      { rewrite map_fmap_union.
+        etransitivity; apply map_union_subseteq_l. }
+      apply map_included_spec.
+      intros k v1 Hv1. exists (S v1).  split; [|lia].
+      by rewrite lookup_fmap Hv1.
+    - eapply (map_included_subseteq_r _ _ (S <$> fs2')).
+      { rewrite map_fmap_union.
+        rewrite (map_union_comm (S <$> fs1') (S <$> fs2')).
+        - etransitivity; apply map_union_subseteq_l.
+        - apply map_disjoint_dom. rewrite !dom_fmap_L.
+          apply map_disjoint_dom in Hdisj.
+          apply map_agree_R_dom in Hle1.
+          apply map_agree_R_dom in Hle2.
+          set_solver. }
+      apply map_included_spec.
+      intros k v1 Hv1. exists (S v1). split; [|lia].
+      by rewrite lookup_fmap Hv1.
+    - rewrite -dom_empty_iff_L in Hne.
+      apply map_agree_R_dom in Hle1.
+      apply map_agree_R_dom in Hle2.
+      apply disjoint_intersection_L.
+      apply map_disjoint_dom in Hdisj.
+      apply map_disjoint_dom in Hdisj'.
+      rewrite dom_union_L.
+      rewrite dom_fmap_L.
+      rewrite -dom_union_L.
+      replace (dom (fs1' ∪ fs2' ∪ fsf') ∖ (dom fs1' ∪ dom fs2'))
+        with (dom fsf') by set_solver.
+      intros ρ Hin1 Hin2.
+      assert (ρ ∈ (dom fs1 ∪ dom fs2)).
+      { rewrite -dom_union_L.
+        rewrite -(dom_fmap_L S).
+        eapply fuel_map_le_live_roles; [| | |apply Hagree'|..].
+        - intros ????. by apply δ1.(ls_map_disj).
+        (* TODO: Fix this by unifying defs *)
+        - rewrite /fuel_map_le_inner map_included_spec.
+          eapply Hfmle.
+        - done.
+        - done.
+        - done.
+        - set_solver. }
+      set_solver.
+    - apply map_agree_R_dom in Hle1.
+      apply map_agree_R_dom in Hle2.
+      apply disjoint_intersection_L.
+      apply map_disjoint_dom in Hdisj.
+      set_solver.
+    - pose proof (not_elem_of_locale_of_from_list es es e)
+        as Hes%Htp; [|apply locales_equiv_refl].
+      apply not_elem_of_dom in Hes. set_solver.
+  Qed.
 
   Lemma model_update_locale_spec_fork extr
-        (auxtr : auxiliary_trace LM) ζ ζf c2 ρs1 ρs2 :
-    model_can_fork_step (trace_last auxtr) ζ
-      (model_update_fork (trace_last auxtr) ζ ζf ρs1 ρs2) →
-    tids_smaller c2.1 (model_update_fork (trace_last auxtr) ζ ζf ρs1 ρs2) →
+        (auxtr : auxiliary_trace LM) ζ ζf c2 ρs1 ρs2 δ2 :
+    δ2.(ls_data) = model_update_fork ζ ζf ρs1 ρs2 (trace_last auxtr) →
+    model_can_fork_step (trace_last auxtr) ζ ζf δ2 →
+    tids_smaller c2.1 δ2 →
     valid_state_evolution_fairness
       (extr :tr[Some ζ]: c2)
-      (auxtr :tr[Silent_step ζ]:
-          (model_update_fork (trace_last auxtr) ζ ζf ρs1 ρs2)).
+      (auxtr :tr[Silent_step ζ]: δ2).
   Proof.
     intros Hstep Htids. destruct c2.
-    split; [done|]. split; [by apply model_can_fork_step_trans|done].
+    split; [done|]. split; [by eapply model_can_fork_step_trans|done].
+  Qed.
+
+  Lemma model_state_interp_has_fuels_agree es δ ζ (fs : gmap (fmrole M) nat) :
+    model_state_interp es δ -∗ has_fuels ζ fs -∗
+    ⌜∃ fs', δ.(ls_map) !! ζ = Some fs' ∧ map_included (≤) fs fs'⌝.
+  Proof.
+    iIntros "Hm Hf".
+    iDestruct "Hm" as (fm [Hfmle _] Hfmdead Htp) "(Hm & Hfm)".
+    iDestruct (has_fuels_agree with "Hfm Hf") as %Hagree.
+    rewrite /fuel_map_le_inner map_included_spec in Hfmle.
+    apply Hfmle in Hagree as (fs'&HSome&Hfs').
+    iPureIntro. by eexists _.
   Qed.
 
   Lemma update_fork_step fs1 fs2 tp1 tp2 (extr : execution_trace Λ)
@@ -1504,16 +2441,27 @@ Section model_state_lemmas.
       model_state_interp tp2 δ2.
   Proof.
     iIntros (Hdom Hdisj Hlast Hstep Hforked) "Hfuel Hm".
+    iDestruct (model_state_interp_has_fuels_agree with "Hm Hfuel")
+      as %(fs'&HSome&Hfs').
+    iAssert (⌜(locale_of tp1 efork) ∉ dom (ls_map (trace_last auxtr))⌝)%I as %Hnin.
+    { destruct Hforked as (?&?&?).
+      iDestruct "Hm" as (fm [_ Hdom'] _ Htp) "[Hm Hfm]".
+      rewrite -Hdom'.
+      iPureIntro. apply not_elem_of_dom. apply Htp.
+      apply locale_step_equiv in Hstep. simpl in *.
+      apply not_elem_of_locale_of_from_list. apply locales_equiv_refl. }
+    pose proof (model_update_fork_valid) as [δ2 Hδ];
+      [by apply elem_of_dom|done|].
     iDestruct (model_state_interp_can_fork_step with "Hm Hfuel") as %Hcan_step;
       [done..|].
     iMod (model_state_interp_fork_update with "Hm Hfuel") as "(Hm&Hf1&Hf2)";
       [done..|].
     iDestruct (model_state_interp_tids_smaller with "Hm") as %Htids.
     iModIntro.
-    iExists (model_update_fork (trace_last auxtr) ζ (locale_of tp1 _) (dom (fs1 ∪ fs2)) (dom fs1)).
+    iExists δ2.
     iFrame "Hm Hf1 Hf2".
     iPureIntro.
-    by apply model_update_locale_spec_fork.
+    by eapply model_update_locale_spec_fork.
   Qed.
 
   Lemma free_roles_inclusion FR fr:
